src/RewriterWf1.v
@@ -35,6 +35,8 @@ Require Import Crypto.Util.CPSNotations.
 Require Import Crypto.Util.Notations.
 Require Import Crypto.Util.HProp.
 Require Import Crypto.Util.Decidable.
+Require Import Crypto.Util.Bool.
+Require Import Crypto.Util.NatUtil.
 Require Crypto.Util.PrimitiveHList.
 Import Coq.Lists.List ListNotations. Local Open Scope list_scope.
 Local Open Scope Z_scope.
@@ -3267,5 +3269,464 @@ Module Compilers.
         Qed.
       End with_interp.
     End Reify.
+
+    Module Import WfTactics.
+      Module Export Settings.
+        Global Strategy -100 [rewrite_rules Compile.rewrite_rules_goodT_curried_cps].
+      End Settings.
+
+      Module Export GoalType.
+        Definition Wf_GoalT (Rewriter : RewriterT) : Prop
+          := forall var1 var2,
+          @Compile.rewrite_rules_goodT
+            ident pattern.ident (@pattern.ident.arg_types) var1 var2
+            (Make.GoalType.rewrite_rules (Rewriter_data Rewriter) _)
+            (Make.GoalType.rewrite_rules (Rewriter_data Rewriter) _).
+      End GoalType.
+
+      Ltac start_good _ :=
+        cbv [Wf_GoalT]; intros;
+        match goal with
+        | [ |- @Compile.rewrite_rules_goodT ?ident ?pident ?pident_arg_types ?var1 ?var2 ?rew1 ?rew2 ]
+          => let H := fresh in
+             pose proof (@Compile.rewrite_rules_goodT_by_curried _ _ _ _ _ rew1 rew2 eq_refl) as H;
+             let data := lazymatch rew1 with Make.GoalType.rewrite_rules ?data _ => data end in
+             let data' := (eval hnf in data) in
+             change data with data' in H;
+             cbv [Make.GoalType.rewrite_rules] in H;
+             let h' := lazymatch type of H with
+                       | context[Compile.rewrite_rules_goodT_curried_cps ?pident_arg_types ?rew1] => head rew1
+                       end in
+             cbv [h' pident_arg_types Compile.rewrite_rules_goodT_curried_cps] in H;
+             (* make [Qed] not take forever by explicitly recording a cast node *)
+             let H' := fresh in
+             pose proof H as H'; clear H;
+             apply H'; clear H'; intros
+        end.
+
+      Ltac fin_wf :=
+        repeat first [ progress intros
+                     | match goal with
+                       | [ |- expr.wf _ (_ @ _) (_ @ _) ] => constructor
+                       | [ |- expr.wf _ (#_) (#_) ] => constructor
+                       | [ |- expr.wf _ ($_) ($_) ] => constructor
+                       | [ |- expr.wf _ (expr.Abs _) (expr.Abs _) ] => constructor; intros
+                       | [ H : @List.In ?T _ ?ls |- _ ] => is_evar ls; unify ls (@nil T); cbn [List.In] in H
+                       | [ |- List.In ?v ?ls ] => is_evar ls; instantiate (1:=cons v _)
+                       end
+                     | progress subst
+                     | progress destruct_head'_or
+                     | progress destruct_head'_False
+                     | progress inversion_sigma
+                     | progress inversion_prod
+                     | assumption
+                     | esplit; revgoals; solve [ fin_wf ]
+                     | econstructor; solve [ fin_wf ]
+                     | progress cbn [List.In fst snd eq_rect] in * ].
+
+      Ltac handle_reified_rewrite_rules :=
+        repeat
+          first [ match goal with
+                  | [ |- option_eq _ ?x ?y ]
+                    => lazymatch x with Some _ => idtac | None => idtac end;
+                       lazymatch y with Some _ => idtac | None => idtac end;
+                       progress cbn [option_eq]
+                  | [ |- UnderLets.wf _ _ (Reify.expr_value_to_rewrite_rule_replacement ?rii1 ?sda _) (Reify.expr_value_to_rewrite_rule_replacement ?rii2 ?sda _) ]
+                    => apply (fun H => @Reify.wf_expr_value_to_rewrite_rule_replacement _ _ _ rii1 rii2 H sda); intros
+                  | [ |- option_eq _ (Compile.reflect_ident_iota _) (Compile.reflect_ident_iota _) ]
+                    => apply Reify.wf_reflect_ident_iota
+                  | [ |- ?x = ?x ] => reflexivity
+                  end
+                | break_innermost_match_step
+                | progress cbv [Compile.wf_maybe_do_again_expr] in *
+                | progress fin_wf ].
+
+      Ltac handle_extra_nbe :=
+        repeat first [ match goal with
+                       | [ |- expr.wf _ (reify_list _) (reify_list _) ] => rewrite expr.wf_reify_list
+                       | [ |- List.Forall2 _ ?x ?x ] => rewrite Forall2_Forall; cbv [Proper]
+                       | [ |- List.Forall2 _ (List.map _ _) (List.map _ _) ] => rewrite Forall2_map_map_iff
+                       | [ |- List.Forall _ (seq _ _) ] => rewrite Forall_seq
+                       end
+                     | progress intros
+                     | progress fin_wf ].
+
+      Ltac handle_extra_arith_rules :=
+        repeat first [ progress cbv [option_eq SubstVarLike.is_var_fst_snd_pair_opp_cast] in *
+                     | break_innermost_match_step
+                     | match goal with
+                       | [ Hwf : Compile.wf_value _ ?x _, H : context[SubstVarLike.is_recursively_var_or_ident _ ?x] |- _ ] => erewrite SubstVarLike.wfT_is_recursively_var_or_ident in H by exact Hwf
+                       end
+                     | congruence
+                     | progress fin_wf ].
+
+
+      Module Export Tactic.
+        Export Settings.
+
+        Ltac prove_good _ :=
+          let do_time := Make.time_if_debug1 in (* eval the level early *)
+          do_time start_good;
+          do_time ltac:(fun _ => handle_reified_rewrite_rules; handle_extra_nbe; handle_extra_arith_rules).
+      End Tactic.
+    End WfTactics.
+
+    Module InterpTactics.
+      Import Crypto.Util.ZRange.
+
+      Module Export GoalType.
+        Local Notation specT rewriter_data
+          := (PrimitiveHList.hlist (@snd bool Prop) (List.skipn (dummy_count rewriter_data) (rewrite_rules_specs rewriter_data)))
+               (only parsing).
+
+        Local Notation rewrite_rules_interp_goodT cast_outside_of_range
+          := (@Compile.rewrite_rules_interp_goodT ident pattern.ident (@pattern.ident.arg_types) (@pattern.ident.to_typed) (@ident.gen_interp cast_outside_of_range)).
+
+        Local Notation "'plet' x := y 'in' z"
+          := (match y return _ with x => z end).
+
+        Definition Interp_GoalT (Rewriter : RewriterT) : Prop
+          := forall (cast_outside_of_range : zrange -> Z -> Z),
+            plet data := Rewriter_data Rewriter in
+              specT data
+              -> rewrite_rules_interp_goodT cast_outside_of_range (Make.GoalType.rewrite_rules data _).
+      End GoalType.
+
+      (** Coq >= 8.9 is much better at [eapply] than Coq <= Coq 8.8 *)
+      Ltac cbv_type_for_Coq88 T :=
+        lazymatch eval hnf in T with
+        | @eq ?T ?A ?B => let A' := (eval cbv [ident.Thunked.bool_rect ident.Thunked.list_case ident.Thunked.list_rect ident.Thunked.nat_rect ident.Thunked.option_rect] in A) in
+                          constr:(@eq T A' B)
+        | forall x : ?A, ?P
+          => let P' := fresh in
+             constr:(forall x : A,
+                        match P return Prop with
+                        | P'
+                          => ltac:(let v := cbv_type_for_Coq88 P' in
+                                   exact v)
+                        end)
+        end.
+      Ltac cbv_for_Coq88_in H :=
+        cbv [ident.Thunked.bool_rect ident.Thunked.list_case ident.Thunked.list_rect ident.Thunked.nat_rect ident.Thunked.option_rect];
+        let T := type of H in
+        let T := cbv_type_for_Coq88 T in
+        change T in H.
+
+      Ltac start_interp_good _ :=
+        cbv [List.skipn Interp_GoalT] in *; intros;
+        lazymatch goal with
+        | [ |- @Compile.rewrite_rules_interp_goodT ?ident ?pident ?pident_arg_types ?pident_to_typed ?ident_interp (Make.GoalType.rewrite_rules ?data ?var) ]
+          => let H := fresh in
+             pose proof (@Compile.rewrite_rules_interp_goodT_by_curried
+                           _ _ _ pident_to_typed ident_interp (Make.GoalType.rewrite_rules data var) (rewrite_rules_specs data)) as H;
+             let data' := (eval hnf in data) in
+             change data with data' in * |- ;
+             cbv [Make.GoalType.rewrite_rules dummy_count rewrite_rules_specs] in * |- ;
+             let h' := lazymatch type of H with context[Compile.rewrite_rules_interp_goodT_curried_cps _ _ _ ?v] => head v end in
+             unfold h' in H at 1;
+             cbv [Compile.rewrite_rules_interp_goodT_curried_cps pident_arg_types pident_to_typed] in H;
+             cbn [snd hd tl projT1 projT2] in H;
+             (* make [Qed] not take forever by explicitly recording a cast node *)
+             let H' := fresh in
+             pose proof H as H'; clear H;
+             apply H'; clear H'
+        end;
+        [ try assumption;
+          cbn [PrimitiveHList.hlist snd];
+          repeat lazymatch goal with
+                 | [ |- PrimitiveProd.Primitive.prod _ _ ] => constructor
+                 | [ |- forall A x, x = x ] => reflexivity
+                 end;
+          try assumption
+        | try match goal with
+              | [ H : PrimitiveHList.hlist _ _ |- _ ] => clear H
+              end;
+          let H := fresh in
+          intro H; hnf in H;
+          repeat first [ progress intros
+                       | match goal with
+                         | [ |- { pf : ?x = ?x | _ } ] => (exists eq_refl)
+                         | [ |- True /\ _ ] => split; [ exact I | ]
+                         | [ |- _ /\ _ ] => split; [ intros; exact I | ]
+                         | [ |- match (if ?b then _ else _) with Some _ => _ | None => _ end ]
+                           => destruct b eqn:?
+                         | [ |- True ] => exact I
+                         end
+                       | progress eta_expand
+                       | progress cbn [eq_rect] in * ];
+          cbn [fst snd base.interp base.base_interp type.interp projT1 projT2 UnderLets.interp expr.interp type.related ident.gen_interp] in *;
+          cbn [fst snd] in *;
+          eta_expand;
+          split_andb;
+          repeat match goal with
+                 | [ H : ?b = true |- _ ] => unique pose proof (@Reflect.reflect_bool _ b _ H)
+                 | [ H : negb _ = false |- _ ] => rewrite Bool.negb_false_iff in H
+                 | [ H : _ = false |- _ ] => rewrite <- Bool.negb_true_iff in H
+                 end;
+          subst; cbv [ident.gets_inlined ident.literal] in *;
+          lazymatch goal with
+          | [ |- ?R ?v ]
+            => let v' := open_constr:(_) in
+               replace v with v';
+               [ | symmetry;
+                   cbv_for_Coq88_in H;
+                   unshelve eapply H; shelve_unifiable;
+                   try eassumption;
+                   try (repeat apply conj; assumption);
+                   try match goal with
+                       | [ |- ?A = ?B ] => first [ is_evar A | is_evar B ]; reflexivity
+                       | [ |- ?T ] => is_evar T; exact I
+                       | [ |- ?P ] (* TODO: Maybe we shouldn't simplify boolean expressions in rewriter reification, since we end up just having to undo it here in a kludgy way....... *)
+                         => apply (proj2 (@Bool.reflect_iff P _ _));
+                            progress rewrite ?Bool.eqb_true_l, ?Bool.eqb_true_r, ?Bool.eqb_false_l, ?Bool.eqb_false_r;
+                            let b := lazymatch goal with |- ?b = true => b end in
+                            apply (proj1 (@Bool.reflect_iff _ b _));
+                            tauto
+                       end ];
+               clear H
+          end;
+          fold (@base.interp) in *
+                                 .. ].
+
+      Ltac recurse_interp_related_step :=
+        let do_replace v :=
+            ((tryif is_evar v then fail else idtac);
+             let v' := open_constr:(_) in
+             let v'' := fresh in
+             cut (v = v'); [ generalize v; intros v'' ?; subst v'' | symmetry ]) in
+        match goal with
+        | _ => progress cbv [expr.interp_related] in *
+        | _ => progress cbn [Compile.reify_expr]
+        | [ |- context[(fst ?x, snd ?x)] ] => progress eta_expand
+        | [ |- context[match ?x with pair a b => _ end] ] => progress eta_expand
+        | [ |- expr.interp_related_gen ?ident_interp ?R ?f ?v ]
+          => do_replace v
+        | [ |- exists (fv : ?T1 -> ?T2) (ev : ?T1),
+              _ /\ _ /\ fv ev = ?x ]
+          => lazymatch T1 with Z => idtac | (Z * Z)%type => idtac end;
+             lazymatch T2 with Z => idtac | (Z * Z)%type => idtac end;
+             first [ do_replace x
+                   | is_evar x; do 2 eexists; repeat apply conj; [ | | reflexivity ] ]
+        | _ => progress intros
+        | [ |- expr.interp_related_gen _ _ _ ?ev ] => is_evar ev; eassumption
+        | [ |- expr.interp_related_gen _ _ (?f @ ?x) ?ev ]
+          => is_evar ev;
+             let fh := fresh in
+             let xh := fresh in
+             set (fh := f); set (xh := x); cbn [expr.interp_related_gen]; subst fh xh;
+             do 2 eexists; repeat apply conj; [ | | reflexivity ]
+        | [ |- expr.interp_related_gen _ _ (expr.Abs ?f) _ ]
+          => let fh := fresh in set (fh := f); cbn [expr.interp_related_gen]; subst fh
+        | [ |- expr.interp_related_gen _ _ (expr.Ident ?idc) ?ev ]
+          => is_evar ev;
+             cbn [expr.interp_related_gen]; apply ident.gen_interp_Proper; reflexivity
+        | [ |- _ = _ :> ?T ]
+          => lazymatch T with
+             | BinInt.Z => idtac
+             | (BinInt.Z * BinInt.Z)%type => idtac
+             end;
+             progress cbn [ident.gen_interp fst snd]
+        | [ |- ?x = ?y ] => tryif first [ has_evar x | has_evar y ] then fail else (progress subst)
+        | [ |- ?x = ?y ] => tryif first [ has_evar x | has_evar y ] then fail else reflexivity
+        | [ |- ?x = ?x ] => tryif has_evar x then fail else reflexivity
+        | [ |- ?ev = _ ] => is_evar ev; reflexivity
+        | [ |- _ = ?ev ] => is_evar ev; reflexivity
+        end.
+
+      (* TODO: MOVE ME? *)
+      Ltac recursive_match_to_case term :=
+        let contains_match x
+            := lazymatch x with
+               | context[match _ with nil => _ | _ => _ end] => true
+               | context[match _ with pair a b => _ end] => true
+               | context[match _ with true => _ | false => _ end] => true
+               | _ => false
+               end in
+        lazymatch term with
+        | context G[match ?ls with nil => ?N | cons x xs => @?C x xs end]
+          => let T := type of N in
+             let term := context G[list_case (fun _ => T) N C ls] in
+             recursive_match_to_case term
+        | context G[match ?v with pair a b => @?P a b end]
+          => let T := lazymatch type of P with forall a b, @?T a b => T end in
+             let term := context G[prod_rect (fun ab => T (fst ab) (snd ab)) P v] in
+             recursive_match_to_case term
+        | context G[match ?b with true => ?t | false => ?f end]
+          => let T := type of t in
+             let term := context G[bool_rect (fun _ => T) t f b] in
+             recursive_match_to_case term
+        | _ => let has_match := contains_match term in
+               match has_match with
+               | true
+                 => let G_f
+                        := match term with
+                           | context G[fun x : ?T => @?f x]
+                             => let has_match := contains_match f in
+                                lazymatch has_match with
+                                | true
+                                  => let f' := fresh in
+                                     let T' := type of f in
+                                     constr:(((fun f' : T' => ltac:(let G' := context G[f'] in exact G')),
+                                              f))
+                                end
+                           end in
+                    lazymatch G_f with
+                    | ((fun f' => ?G), (fun x : ?T => ?f))
+                      => let x' := fresh in
+                         let rep := constr:(fun x' : T
+                                            => ltac:(let f := constr:(match x' with x => f end) in
+                                                     let f := recursive_match_to_case f in
+                                                     exact f)) in
+                         let term := constr:(match rep with f' => G end) in
+                         recursive_match_to_case term
+                    end
+               | false
+                 => term
+               end
+        end.
+      Ltac recursive_match_to_case_in_goal :=
+        let G := match goal with |- ?G => G end in
+        let G := recursive_match_to_case G in
+        change G.
+
+      Ltac preprocess_step :=
+        first [ progress cbv [expr.interp_related respectful ident.literal ident.eagerly] in *
+              | progress cbn [fst snd base.interp base.base_interp Compile.value'] in *
+              | progress intros
+              | progress subst
+              | match goal with
+                | [ |- context[match _ with nil => _ | _ => _ end] ] => progress recursive_match_to_case_in_goal
+                | [ |- context[match _ with pair a b => _ end] ] => progress recursive_match_to_case_in_goal
+                | [ |- context[match _ with true => _ | false => _ end] ] => progress recursive_match_to_case_in_goal
+                | [ |- context[match invert_expr.reflect_list ?ls with _ => _ end] ]
+                  => destruct (invert_expr.reflect_list ls) eqn:?
+                | [ |- context G[expr.interp_related_gen ?ident_interp (fun t : ?T => ?vii t ?b)] ]
+                  => progress change (fun t : T => vii t b) with (fun t : T => @Compile.value_interp_related _ ident_interp t b)
+                end ].
+      Ltac preprocess := repeat preprocess_step.
+      Ltac handle_extra_nbe :=
+        repeat match goal with
+               | [ |- UnderLets.interp_related _ _ (UnderLets.Base (expr.Ident _)) _ ]
+                 => cbn [UnderLets.interp_related UnderLets.interp_related_gen expr.interp_related_gen ident.gen_interp type.related]; reflexivity
+               | [ |- UnderLets.interp_related _ _ (UnderLets.Base (reify_list _)) _ ]
+                 => cbn [UnderLets.interp_related UnderLets.interp_related_gen]; rewrite expr.reify_list_interp_related_gen_iff
+               | [ |- UnderLets.interp_related _ _ (UnderLets.Base (_, _)%expr) ?x ]
+                 => cbn [UnderLets.interp_related UnderLets.interp_related_gen];
+                    recurse_interp_related_step;
+                    [ recurse_interp_related_step
+                    | lazymatch x with
+                      | (_, _) => reflexivity
+                      | _ => etransitivity; [ | symmetry; apply surjective_pairing ]; reflexivity
+                      end ];
+                    [ | reflexivity ]; cbn [fst snd];
+                    recurse_interp_related_step; [ recurse_interp_related_step | reflexivity ]
+               | [ |- List.Forall2 _ (List.map _ _) _ ]
+                 => rewrite Forall2_map_l_iff
+               | [ |- List.Forall2 _ ?x ?x ] => rewrite Forall2_Forall; cbv [Proper]
+               | [ |- List.Forall _ _ ] => rewrite Forall_forall; intros
+               | [ |- expr.interp_related_gen _ _ (expr.Ident _) _ ]
+                 => cbn [expr.interp_related_gen ident.gen_interp type.related]; reflexivity
+               end.
+      Ltac fin_tac :=
+        repeat first [ assumption
+                     | progress change S with Nat.succ
+                     | progress cbn [base.interp base.base_interp type.interp] in *
+                     | progress fold (@type.interp _ base.interp)
+                     | progress fold (@base.interp)
+                     | progress subst
+                     | progress cbv [respectful ident.Thunked.bool_rect ident.Thunked.list_case ident.Thunked.option_rect pointwise_relation]
+                     | progress intros
+                     | solve [ auto ]
+                     | match goal with
+                       | [ |- ?x = ?x ] => reflexivity
+                       | [ |- list_rect _ _ _ _ = ident.Thunked.list_rect _ _ _ _ ]
+                         => cbv [ident.Thunked.list_rect]; apply list_rect_Proper; cbv [pointwise_relation]; intros
+                       | [ |- list_rect (fun _ => ?A -> ?B) _ _ _ _ = list_rect _ _ _ _ _ ]
+                         => apply list_rect_arrow_Proper; cbv [respectful]; intros
+                       | [ |- nat_rect _ _ _ _ = ident.Thunked.nat_rect _ _ _ _ ]
+                         => apply nat_rect_Proper_nondep; cbv [respectful]
+                       | [ |- nat_rect (fun _ => ?A -> ?B) _ _ _ _ = nat_rect _ _ _ _ _ ]
+                         => apply (@nat_rect_Proper_nondep_gen (A -> B) (eq ==> eq)%signature); cbv [respectful]; intros
+                       | [ |- list_case _ _ _ ?ls = list_case _ _ _ ?ls ]
+                         => is_var ls; destruct ls; cbn [list_case]
+                       | [ |- bool_rect _ _ _ ?b = bool_rect _ _ _ ?b ]
+                         => is_var b; destruct b; cbn [bool_rect]
+                       | [ |- _ = ident.cast2 _ _ _ ] => cbv [ident.cast2]; break_innermost_match
+                       end ].
+      Ltac handle_reified_rewrite_rules_interp :=
+        repeat first [ assumption
+                     | match goal with
+                       | [ cast_outside_of_range : zrange -> Z -> Z |- UnderLets.interp_related _ _ (Reify.expr_value_to_rewrite_rule_replacement _ ?sda _) _ ]
+                         => apply (@Reify.expr_value_to_rewrite_rule_replacement_interp_related cast_outside_of_range _ (@Reify.reflect_ident_iota_interp_related cast_outside_of_range) sda)
+
+                       | [ |- UnderLets.interp_related_gen ?ii ?R (UnderLets.Base (#ident.list_rect @ _ @ _ @ _)%expr) (@list_rect ?A (fun _ => ?P) ?N ?C ?ls) ]
+                         => progress change (@list_rect A (fun _ => P) N C ls) with (@ident.Thunked.list_rect A P (fun _ => N) C ls)
+                       | [ |- expr.interp_related_gen ?ii ?R (#ident.list_rect @ _ @ _ @ _)%expr (@list_rect ?A (fun _ => ?P) ?N ?C ?ls) ]
+                         => progress change (@list_rect A (fun _ => P) N C ls) with (@ident.Thunked.list_rect A P (fun _ => N) C ls)
+                       | [ |- expr.interp_related_gen ?ii ?R (#ident.eager_list_rect @ _ @ _ @ _)%expr (@list_rect ?A (fun _ => ?P) ?N ?C ?ls) ]
+                         => progress change (@list_rect A (fun _ => P) N C ls) with (@ident.Thunked.list_rect A P (fun _ => N) C ls)
+                       | [ |- expr.interp_related_gen ?ii ?R (#ident.list_case @ _ @ _ @ _)%expr (@list_case ?A (fun _ => ?P) ?N ?C ?ls) ]
+                         => progress change (@list_case A (fun _ => P) N C ls) with (@ident.Thunked.list_case A P (fun _ => N) C ls)
+                       | [ |- expr.interp_related_gen ?ii ?R (#ident.nat_rect @ _ @ _ @ _)%expr (@nat_rect (fun _ => ?P) ?N ?C ?ls) ]
+                         => progress change (@nat_rect (fun _ => P) N C ls) with (@ident.Thunked.nat_rect P (fun _ => N) C ls)
+                       | [ |- expr.interp_related_gen ?ii ?R (#ident.eager_nat_rect @ _ @ _ @ _)%expr (@nat_rect (fun _ => ?P) ?N ?C ?ls) ]
+                         => progress change (@nat_rect (fun _ => P) N C ls) with (@ident.Thunked.nat_rect P (fun _ => N) C ls)
+                       | [ |- expr.interp_related_gen ?ii ?R (#ident.bool_rect @ _ @ _ @ _)%expr (@bool_rect (fun _ => ?P) ?T ?F ?b) ]
+                         => progress change (@bool_rect (fun _ => P) T F b) with (@ident.Thunked.bool_rect P (fun _ => T) (fun _ => F) b)
+                       | [ |- expr.interp_related_gen ?ii ?R (#ident.option_rect @ _ @ _ @ _)%expr (@option_rect ?A (fun _ => ?P) ?S ?N ?o) ]
+                         => progress change (@option_rect A (fun _ => P) S N o) with (@ident.Thunked.option_rect A P S (fun _ => N) o)
+
+                       | [ |- match ?x with pair _ _ => _ end = prod_rect _ _ _ ]
+                         => cbv [prod_rect]; eta_expand
+
+                       | [ |- expr.interp_related_gen _ _ (expr.Var _) _ ]
+                         => cbn [expr.interp_related_gen]
+                       | [ |- expr.interp_related_gen _ _ (expr.Ident _) _ ]
+                         => cbn [expr.interp_related_gen ident.gen_interp type.related]; fin_tac
+                       | [ |- expr.interp_related_gen _ _ (expr.Abs ?f) _ ]
+                         => let fh := fresh in set (fh := f); cbn [expr.interp_related_gen]; subst fh; cbv beta; intros
+                       | [ |- expr.interp_related_gen _ _ (expr.LetIn ?v ?f) (LetIn.Let_In ?V ?F) ]
+                         => let vh := fresh in
+                            set (vh := v);
+                            let fh := fresh in
+                            set (fh := f);
+                            cbn [expr.interp_related_gen]; subst fh vh; cbv beta;
+                            exists F, V; repeat apply conj; intros
+                       | [ |- expr.interp_related_gen _ _ (?f @ ?x)%expr (?F ?X) ]
+                         => let fh := fresh in
+                            set (fh := f);
+                            let xh := fresh in
+                            set (xh := x);
+                            cbn [expr.interp_related_gen]; subst fh xh;
+                            exists F, X; repeat apply conj; [ | | reflexivity ]
+
+                       | [ |- _ = _ ] => solve [ fin_tac ]
+                       | [ |- type.eqv _ _ ] => cbn [ident.gen_interp type.related]; cbv [respectful]; intros; subst
+                       end
+                     | progress repeat (do 2 eexists; repeat apply conj; [ | | reflexivity ]) ].
+
+      Module Export Tactic.
+        Ltac prove_interp_good _ :=
+          let do_time := Make.time_if_debug1 in (* eval the level early *)
+          do_time start_interp_good;
+          do_time ltac:(fun _ => preprocess; handle_extra_nbe; handle_reified_rewrite_rules_interp).
+      End Tactic.
+    End InterpTactics.
+
+    Module GoalType.
+      Record VerifiedRewriter :=
+        {
+          Rewriter : RewriterT;
+          RewriterRulesWf : WfTactics.GoalType.Wf_GoalT Rewriter;
+          RewriterRulesInterp : InterpTactics.GoalType.Interp_GoalT Rewriter;
+          Wf_Rewrite : forall {t} e (Hwf : Wf e), Wf (@Rewrite Rewriter t e);
+          Interp_gen_Rewrite
+          : forall {cast_outside_of_range t} e (Hwf : Wf e),
+              expr.Interp (@ident.gen_interp cast_outside_of_range) (@Rewrite Rewriter t e)
+              == expr.Interp (@ident.gen_interp cast_outside_of_range) e;
+          Interp_Rewrite
+          : forall {t} e (Hwf : Wf e), Interp (@Rewrite Rewriter t e) == Interp e
+        }.
+    End GoalType.
   End RewriteRules.
 End Compilers.
