src/Rewriter.v
@@ -13,7 +13,6 @@ Require Import Crypto.Util.ZUtil.Notations.
 Require Import Crypto.Util.Tactics.ConstrFail.
 Require Crypto.Util.PrimitiveProd.
 Require Crypto.Util.PrimitiveHList.
-Require Import Crypto.RewriterRules.
 Require Import Crypto.Language.
 Require Import Crypto.UnderLets.
 Require Import Crypto.GENERATEDIdentifiersWithoutTypes.
@@ -1716,7 +1715,11 @@ Module Compilers.
       Ltac equation_to_parts' lem side_conditions :=
         lazymatch lem with
         | ?H -> ?P
-          => let H := prop_to_bool H in
+          => let __ := lazymatch type of H with
+                       | Prop => constr:(I)
+                       | ?T => constr_fail_with ltac:(fun _ => fail 1 "Invalid non-Prop non-dependent hypothesis of type" H ":" T "when reifying a lemma of type" lem)
+                       end in
+             let H := prop_to_bool H in
              let side_conditions := push_side_conditions H side_conditions in
              equation_to_parts' P side_conditions
         | forall x : ?T, ?P
@@ -2435,12 +2438,16 @@ Module Compilers.
         | _ => check_debug_level_then_Set ()
         end.
 
+      Definition pident_unify_unknown := @pattern.ident.unify.
+      Definition invert_bind_args_unknown := @pattern.Raw.ident.invert_bind_args.
+
       Module Export GoalType.
         Record rewriter_dataT :=
           Build_rewriter_dataT'
             {
               rewrite_rules_specs : list (bool * Prop);
               dummy_count : nat;
+              dtree : @Compile.decision_tree pattern.Raw.ident;
 
               rewrite_rules : forall var, @Compile.rewrite_rulesT ident var pattern.ident (@pattern.ident.arg_types) ;
               all_rewrite_rules (* adjusted version *) : _;
@@ -2448,9 +2455,11 @@ Module Compilers.
 
               default_fuel : nat;
 
-              rewrite_head0 : forall var (do_again : forall t, @defaults.expr (@Compile.value _ ident var) (type.base t) -> @UnderLets.UnderLets _ ident var (@defaults.expr var (type.base t)))
+              rewrite_head0
+              := (fun var
+                  => @Compile.assemble_identifier_rewriters ident var (@pattern.ident.eta_ident_cps) (@pattern.ident) (@pattern.ident.arg_types) (@pattern.ident.unify) pident_unify_unknown pattern.Raw.ident (@pattern.Raw.ident.full_types) (@pattern.Raw.ident.invert_bind_args) invert_bind_args_unknown (@pattern.Raw.ident.type_of) (@pattern.Raw.ident.to_typed) pattern.Raw.ident.is_simple dtree (all_rewrite_rules var));
+              rewrite_head (* adjusted version *) : forall var (do_again : forall t, @defaults.expr (@Compile.value _ ident var) (type.base t) -> @UnderLets.UnderLets _ ident var (@defaults.expr var (type.base t)))
                                      t (idc : ident t), @Compile.value_with_lets base.type ident var t;
-              rewrite_head (* adjusted version *) : _;
               rewrite_head_eq : rewrite_head = rewrite_head0
             }.
       End GoalType.
@@ -2473,94 +2482,95 @@ Module Compilers.
         | _ => constr_fail_with ltac:(fun _ => fail 1 "Invalid value for include_interp (must be either true or false):" include_interp)
         end.
 
-      Definition pident_unify_unknown := @pattern.ident.unify.
-      Definition invert_bind_args_unknown := @pattern.Raw.ident.invert_bind_args.
+      Ltac time_if_debug1 :=
+        let lvl := rewriter_assembly_debug_level in
+        lazymatch lvl with
+        | O => ltac:(fun tac => tac ())
+        | S _ => ltac:(fun tac => time tac ())
+        | ?v => ltac:(fun tac => fail 0 "Invalid non-nat rewriter_assembly_debug_level" v)
+        end.
+      Ltac time_tac_in_constr_if_debug1 tac :=
+        constr:(ltac:(time_if_debug1 ltac:(fun _ => idtac; let v := tac () in exact v))).
 
       Ltac make_rewrite_head1 rewrite_head0 pr2_rewrite_rules :=
-        let rewrite_head1
-            := (eval cbv -[pr2_rewrite_rules
-                             base.interp base.try_make_transport_cps
-                             type.try_make_transport_cps
-                             pattern.type.unify_extracted
-                             Compile.option_type_type_beq
-                             Let_In Option.sequence Option.sequence_return
-                             UnderLets.splice UnderLets.to_expr
-                             Compile.option_bind' pident_unify_unknown invert_bind_args_unknown Compile.normalize_deep_rewrite_rule
-                             Compile.reflect UnderLets.reify_and_let_binds_base_cps Compile.reify Compile.reify_and_let_binds_cps
-                             Compile.value'
-                             SubstVarLike.is_var_fst_snd_pair_opp_cast
-                          ] in rewrite_head0) in
-        let rewrite_head1
-            := (eval cbn [type.try_make_transport_cps base.try_make_transport_cps base.try_make_base_transport_cps]
-                 in rewrite_head1) in
-        rewrite_head1.
-      Ltac timed_make_rewrite_head1 rewrite_head0 pr2_rewrite_rules :=
-        constr:(ltac:(time (idtac; let v := make_rewrite_head1 rewrite_head0 pr2_rewrite_rules in exact v))).
+        time_tac_in_constr_if_debug1
+          ltac:(fun _
+                => let rewrite_head1
+                       := (eval cbv -[pr2_rewrite_rules
+                                        base.interp base.try_make_transport_cps
+                                        type.try_make_transport_cps
+                                        pattern.type.unify_extracted
+                                        Compile.option_type_type_beq
+                                        Let_In Option.sequence Option.sequence_return
+                                        UnderLets.splice UnderLets.to_expr
+                                        Compile.option_bind' pident_unify_unknown invert_bind_args_unknown Compile.normalize_deep_rewrite_rule
+                                        Compile.reflect UnderLets.reify_and_let_binds_base_cps Compile.reify Compile.reify_and_let_binds_cps
+                                        Compile.value'
+                                        SubstVarLike.is_var_fst_snd_pair_opp_cast
+                                     ] in rewrite_head0) in
+                   let rewrite_head1
+                       := (eval cbn [type.try_make_transport_cps base.try_make_transport_cps base.try_make_base_transport_cps]
+                            in rewrite_head1) in
+                   rewrite_head1).
       Ltac make_rewrite_head2 rewrite_head1 pr2_rewrite_rules :=
-        (eval cbv [id
-                     pr2_rewrite_rules
-                     projT1 projT2
-                     cpsbind cpscall cps_option_bind cpsreturn
-                     PrimitiveProd.Primitive.fst PrimitiveProd.Primitive.snd
-                     pattern.type.subst_default pattern.base.subst_default pattern.base.lookup_default
-                     PositiveMap.add PositiveMap.find PositiveMap.empty
-                     PositiveSet.rev PositiveSet.rev_append
-                     pattern.ident.arg_types
-                     Compile.eval_decision_tree
-                     Compile.eval_rewrite_rules
-                     Compile.expr_of_rawexpr
-                     Compile.normalize_deep_rewrite_rule
-                     Compile.option_bind' pident_unify_unknown invert_bind_args_unknown Compile.normalize_deep_rewrite_rule
-                     (*Compile.reflect*)
-                     (*Compile.reify*)
-                     Compile.reveal_rawexpr_cps
-                     Compile.reveal_rawexpr_cps_gen
-                     Compile.rew_should_do_again
-                     Compile.rew_with_opt
-                     Compile.rew_under_lets
-                     Compile.rew_replacement
-                     Compile.rValueOrExpr
-                     Compile.swap_list
-                     Compile.type_of_rawexpr
-                     Compile.option_type_type_beq
-                     Compile.value
-                     (*Compile.value'*)
-                     Compile.value_of_rawexpr
-                     Compile.value_with_lets
-                     ident.smart_Literal
-                     type.try_transport_cps
-                     (*rlist_rect rwhen rwhenl*)
-                  ] in rewrite_head1).
-      Ltac timed_make_rewrite_head2 rewrite_head1 pr2_rewrite_rules :=
-        constr:(ltac:(time (idtac; let v := make_rewrite_head2 rewrite_head1 pr2_rewrite_rules in exact v))).
+        time_tac_in_constr_if_debug1
+          ltac:(fun _
+                => (eval cbv [id
+                                pr2_rewrite_rules
+                                projT1 projT2
+                                cpsbind cpscall cps_option_bind cpsreturn
+                                PrimitiveProd.Primitive.fst PrimitiveProd.Primitive.snd
+                                pattern.type.subst_default pattern.base.subst_default pattern.base.lookup_default
+                                PositiveMap.add PositiveMap.find PositiveMap.empty
+                                PositiveSet.rev PositiveSet.rev_append
+                                pattern.ident.arg_types
+                                Compile.eval_decision_tree
+                                Compile.eval_rewrite_rules
+                                Compile.expr_of_rawexpr
+                                Compile.normalize_deep_rewrite_rule
+                                Compile.option_bind' pident_unify_unknown invert_bind_args_unknown Compile.normalize_deep_rewrite_rule
+                                (*Compile.reflect*)
+                                (*Compile.reify*)
+                                Compile.reveal_rawexpr_cps
+                                Compile.reveal_rawexpr_cps_gen
+                                Compile.rew_should_do_again
+                                Compile.rew_with_opt
+                                Compile.rew_under_lets
+                                Compile.rew_replacement
+                                Compile.rValueOrExpr
+                                Compile.swap_list
+                                Compile.type_of_rawexpr
+                                Compile.option_type_type_beq
+                                Compile.value
+                                (*Compile.value'*)
+                                Compile.value_of_rawexpr
+                                Compile.value_with_lets
+                                ident.smart_Literal
+                                type.try_transport_cps
+                                (*rlist_rect rwhen rwhenl*)
+                             ] in rewrite_head1)).
       Ltac make_rewrite_head3 rewrite_head2 :=
-        (eval cbn [id
-                     cpsbind cpscall cps_option_bind cpsreturn
-                     Compile.reify Compile.reify_and_let_binds_cps Compile.reflect Compile.value'
-                     Option.sequence Option.sequence_return Option.bind
-                     UnderLets.reify_and_let_binds_base_cps
-                     UnderLets.splice UnderLets.splice_list UnderLets.to_expr
-                     base.interp base.base_interp
-                     base.type.base_beq option_beq
-                     type.try_make_transport_cps base.try_make_transport_cps base.try_make_base_transport_cps
-                     Datatypes.fst Datatypes.snd
-                  ] in rewrite_head2).
-      Ltac timed_make_rewrite_head3 rewrite_head2 :=
-        constr:(ltac:(time (idtac; let v := make_rewrite_head3 rewrite_head2 in exact v))).
+        time_tac_in_constr_if_debug1
+          ltac:(fun _
+                => (eval cbn [id
+                                cpsbind cpscall cps_option_bind cpsreturn
+                                Compile.reify Compile.reify_and_let_binds_cps Compile.reflect Compile.value'
+                                Option.sequence Option.sequence_return Option.bind
+                                UnderLets.reify_and_let_binds_base_cps
+                                UnderLets.splice UnderLets.splice_list UnderLets.to_expr
+                                base.interp base.base_interp
+                                base.type.base_beq option_beq
+                                type.try_make_transport_cps base.try_make_transport_cps base.try_make_base_transport_cps
+                                Datatypes.fst Datatypes.snd
+                             ] in rewrite_head2)).
       Ltac make_rewrite_head' rewrite_head0 pr2_rewrite_rules :=
         let rewrite_head1 := make_rewrite_head1 rewrite_head0 pr2_rewrite_rules in
         let rewrite_head2 := make_rewrite_head2 rewrite_head1 pr2_rewrite_rules in
         let rewrite_head3 := make_rewrite_head3 rewrite_head2 in
         rewrite_head3.
-      Ltac timed_make_rewrite_head' rewrite_head0 pr2_rewrite_rules :=
-        let rewrite_head1 := timed_make_rewrite_head1 rewrite_head0 pr2_rewrite_rules in
-        let rewrite_head2 := timed_make_rewrite_head2 rewrite_head1 pr2_rewrite_rules in
-        let rewrite_head3 := timed_make_rewrite_head3 rewrite_head2 in
-        rewrite_head3.
 
       Ltac make_rewrite_head rewrite_head0 pr2_rewrite_rules :=
         let rewrite_head := fresh "rewrite_head" in
-        let lvl := rewriter_assembly_debug_level in
         let var := fresh "var" in
         let do_again := fresh "do_again" in
         let t := fresh "t" in
@@ -2572,10 +2582,7 @@ Module Compilers.
               => ltac:(
                    let rewrite_head0 := constr:(rewrite_head0 var do_again t idc) in
                    let pr2_rewrite_rules := head pr2_rewrite_rules in
-                   let v := lazymatch lvl with
-                            | O => make_rewrite_head' rewrite_head0 pr2_rewrite_rules
-                            | S _ => timed_make_rewrite_head' rewrite_head0 pr2_rewrite_rules
-                            end in
+                   let v := make_rewrite_head' rewrite_head0 pr2_rewrite_rules in
                    exact v)) in
         cache_term v rewrite_head.
 
@@ -2605,187 +2612,56 @@ Module Compilers.
                  rewrite_head0 in
         let __ := debug1 ltac:(fun _ => idtac "Reducing rewrite_head...") in
         let rewrite_head := make_rewrite_head rewrite_head0 pr2_rewrite_rules in
-        refine (@Build_rewriter_dataT'
-                  specs dummy_count
+        constr:(@Build_rewriter_dataT'
+                  specs dummy_count dtree
                   rewrite_rules all_rewrite_rules eq_refl
                   default_fuel
-                  rewrite_head0 rewrite_head eq_refl).
+                  (*rewrite_head0*) rewrite_head eq_refl).
 
       Module Export Tactic.
-        Global Arguments base.try_make_base_transport_cps _ !_ !_.
-        Global Arguments base.try_make_transport_cps _ !_ !_.
-        Global Arguments type.try_make_transport_cps _ _ _ !_ !_.
-        Global Arguments Option.sequence A !v1 v2.
-        Global Arguments Option.sequence_return A !v1 v2.
-        Global Arguments Option.bind A B !_ _.
-        Global Arguments pattern.Raw.ident.invert_bind_args t !_ !_.
-        Global Arguments base.type.base_beq !_ !_.
-        Global Arguments id / .
+        Module Export Settings.
+          Global Arguments base.try_make_base_transport_cps _ !_ !_.
+          Global Arguments base.try_make_transport_cps _ !_ !_.
+          Global Arguments type.try_make_transport_cps _ _ _ !_ !_.
+          Global Arguments Option.sequence A !v1 v2.
+          Global Arguments Option.sequence_return A !v1 v2.
+          Global Arguments Option.bind A B !_ _.
+          Global Arguments pattern.Raw.ident.invert_bind_args t !_ !_.
+          Global Arguments base.type.base_beq !_ !_.
+          Global Arguments id / .
+        End Settings.
 
         Tactic Notation "make_rewriter_data" constr(include_interp) constr(specs) :=
-          Build_rewriter_dataT include_interp specs.
+          let res := Build_rewriter_dataT include_interp specs in refine res.
       End Tactic.
     End Make.
     Export Make.GoalType.
     Import Make.Tactic.
 
-    Definition nbe_rewriter_data : rewriter_dataT.
-    Proof. make_rewriter_data true nbe_rewrite_rulesT. Defined.
+    Module Export GoalType.
+      Record RewriterT :=
+        {
+          Rewriter_data : rewriter_dataT;
+          Rewrite : forall {t} (e : expr.Expr (ident:=ident) t), expr.Expr (ident:=ident) t;
+          Rewrite_eq : @Rewrite = @Make.Rewrite Rewriter_data
+        }.
+    End GoalType.
 
-    Definition arith_rewriter_data (max_const_val : Z) : rewriter_dataT.
-    Proof. make_rewriter_data false (arith_rewrite_rulesT max_const_val). Defined.
+    Ltac Build_RewriterT include_interp specs :=
+      let rewriter_data := fresh "rewriter_data" in
+      let data := Make.Build_rewriter_dataT include_interp specs in
+      let Rewrite_name := fresh "Rewriter" in
+      let Rewrite := (eval cbv [Make.Rewrite rewrite_head default_fuel] in (@Make.Rewrite data)) in
+      let Rewrite := cache_term Rewrite Rewrite_name in
+      constr:(@Build_RewriterT data Rewrite eq_refl).
 
-    Definition arith_with_casts_rewriter_data : rewriter_dataT.
-    Proof. make_rewriter_data false arith_with_casts_rewrite_rulesT. Defined.
+    Module Export Tactic.
+      Module Export Settings.
+        Export Make.Tactic.Settings.
+      End Settings.
 
-    Definition strip_literal_casts_rewriter_data : rewriter_dataT.
-    Proof. make_rewriter_data false strip_literal_casts_rewrite_rulesT. Defined.
-
-    Definition fancy_rewriter_data
-               (invert_low invert_high : Z (*log2wordmax*) -> Z -> option Z)
-      : rewriter_dataT.
-    Proof. make_rewriter_data false fancy_rewrite_rulesT. Defined.
-
-    Definition fancy_with_casts_rewriter_data
-               (invert_low invert_high : Z (*log2wordmax*) -> Z -> option Z)
-               (value_range flag_range : zrange)
-      : rewriter_dataT.
-    Proof. make_rewriter_data false (fancy_with_casts_rewrite_rulesT invert_low invert_high value_range flag_range). Defined.
-
-    Module RewriterPrintingNotations.
-      Arguments base.try_make_transport_cps {P} t1 t2 {_} _.
-      Arguments type.try_make_transport_cps {base_type _ P} t1 t2 {_} _.
-      Export pattern.Raw.ident.
-      Export GENERATEDIdentifiersWithoutTypes.Compilers.pattern.Raw.
-      Export GENERATEDIdentifiersWithoutTypes.Compilers.pattern.
-      Export UnderLets.
-      Export Compilers.ident.
-      Export Language.Compilers.
-      Export Language.Compilers.defaults.
-      Export PrimitiveSigma.Primitive.
-      Notation "'llet' x := v 'in' f" := (Let_In v (fun x => f)).
-      Notation "x <- 'type.try_make_transport_cps' t1 t2 ; f" := (type.try_make_transport_cps t1 t2 (fun y => match y with Datatypes.Some x => f | Datatypes.None => Datatypes.None end)) (at level 70, t1 at next level, t2 at next level, right associativity, format "'[v' x  <-  'type.try_make_transport_cps'  t1  t2 ; '/' f ']'").
-      Notation "x <- 'base.try_make_transport_cps' t1 t2 ; f" := (base.try_make_transport_cps t1 t2 (fun y => match y with Datatypes.Some x => f | Datatypes.None => Datatypes.None end)) (at level 70, t1 at next level, t2 at next level, right associativity, format "'[v' x  <-  'base.try_make_transport_cps'  t1  t2 ; '/' f ']'").
-    End RewriterPrintingNotations.
-
-    (* For printing *)
-    Local Arguments base.try_make_transport_cps {P} t1 t2 {_} _.
-    Local Arguments type.try_make_transport_cps {base_type _ P} t1 t2 {_} _.
-    Local Arguments option {_}.
-    Local Arguments UnderLets.UnderLets {_ _ _}.
-    Local Arguments expr.expr {_ _ _}.
-    Local Notation ℤ := base.type.Z.
-    Local Notation ℕ := base.type.nat.
-    Local Notation bool := base.type.bool.
-    Local Notation unit := base.type.unit.
-    Local Notation list := base.type.list.
-    Local Notation "x" := (type.base x) (only printing, at level 9).
-
-    Section red_fancy.
-      Context (invert_low invert_high : Z (*log2wordmax*) -> Z -> @option Z).
-
-      Local Definition fancy_rewrite_head
-        := Eval hnf in rewrite_head (fancy_rewriter_data invert_low invert_high).
-
-      Local Set Printing Depth 1000000.
-      Local Set Printing Width 200.
-      Import RewriterPrintingNotations.
-      Redirect "fancy_rewrite_head" Print fancy_rewrite_head.
-    End red_fancy.
-    Section red_fancy_with_casts.
-      Context (invert_low invert_high : Z (*log2wordmax*) -> Z -> @option Z)
-              (value_range flag_range : zrange).
-
-      Local Definition fancy_with_casts_rewrite_head
-        := Eval hnf in rewrite_head (fancy_with_casts_rewriter_data invert_low invert_high value_range flag_range).
-
-      Local Set Printing Depth 1000000.
-      Local Set Printing Width 200.
-      Import RewriterPrintingNotations.
-      Redirect "fancy_with_casts_rewrite_head" Print fancy_with_casts_rewrite_head.
-    End red_fancy_with_casts.
-    Section red_nbe.
-      Local Definition nbe_rewrite_head
-        := Eval hnf in rewrite_head nbe_rewriter_data.
-
-      Local Set Printing Depth 1000000.
-      Local Set Printing Width 200.
-      Import RewriterPrintingNotations.
-      Redirect "nbe_rewrite_head" Print nbe_rewrite_head.
-    End red_nbe.
-
-    Section red_arith.
-      Context (max_const_val : Z).
-
-      Local Definition arith_rewrite_head
-        := Eval hnf in rewrite_head (arith_rewriter_data max_const_val).
-
-      Local Set Printing Depth 1000000.
-      Local Set Printing Width 200.
-      Import RewriterPrintingNotations.
-      Redirect "arith_rewrite_head" Print arith_rewrite_head.
-    End red_arith.
-
-    Section red_arith_with_casts.
-      Local Definition arith_with_casts_rewrite_head
-        := Eval hnf in rewrite_head arith_with_casts_rewriter_data.
-
-      Local Set Printing Depth 1000000.
-      Local Set Printing Width 200.
-      Import RewriterPrintingNotations.
-      Redirect "arith_with_casts_rewrite_head" Print arith_with_casts_rewrite_head.
-    End red_arith_with_casts.
-
-    Section red_strip_literal_casts.
-      Local Definition strip_literal_casts_rewrite_head
-        := Eval hnf in rewrite_head strip_literal_casts_rewriter_data.
-
-      Local Set Printing Depth 1000000.
-      Local Set Printing Width 200.
-      Import RewriterPrintingNotations.
-      Redirect "strip_literal_casts_rewrite_head" Print strip_literal_casts_rewrite_head.
-    End red_strip_literal_casts.
-
-    Local Ltac unfold_Rewrite Rewrite :=
-      let h := head Rewrite in
-      let Rewrite := (eval cbv [h] in Rewrite) in
-      let data := lazymatch Rewrite with context[@Make.Rewrite ?data] => head data end in
-      (eval cbv [Make.Rewrite rewrite_head default_fuel data] in Rewrite).
-    Local Notation unfold_Rewrite Rewrite :=
-      (ltac:(let v := unfold_Rewrite Rewrite in
-             exact v)) (only parsing).
-
-    Definition RewriteNBE_folded := @Make.Rewrite nbe_rewriter_data.
-    Definition RewriteNBE {t} (e : expr.Expr (ident:=ident) t) : expr.Expr (ident:=ident) t
-      := unfold_Rewrite (@RewriteNBE_folded t e).
-    Definition RewriteArith_folded (max_const_val : Z) := @Make.Rewrite (arith_rewriter_data max_const_val).
-    Definition RewriteArith (max_const_val : Z) {t} (e : expr.Expr (ident:=ident) t) : expr.Expr (ident:=ident) t
-      := unfold_Rewrite (@RewriteArith_folded max_const_val t e).
-    Definition RewriteArithWithCasts_folded := @Make.Rewrite arith_with_casts_rewriter_data.
-    Definition RewriteArithWithCasts {t} (e : expr.Expr (ident:=ident) t) : expr.Expr (ident:=ident) t
-      := unfold_Rewrite (@RewriteArithWithCasts_folded t e).
-    Definition RewriteStripLiteralCasts_folded := @Make.Rewrite strip_literal_casts_rewriter_data.
-    Definition RewriteStripLiteralCasts {t} (e : expr.Expr (ident:=ident) t) : expr.Expr (ident:=ident) t
-      := unfold_Rewrite (@RewriteStripLiteralCasts_folded t e).
-    Definition RewriteToFancy_folded
-               (invert_low invert_high : Z (*log2wordmax*) -> Z -> @option Z)
-      := @Make.Rewrite (fancy_rewriter_data invert_low invert_high).
-    Definition RewriteToFancy
-               (invert_low invert_high : Z (*log2wordmax*) -> Z -> @option Z)
-               {t} (e : expr.Expr (ident:=ident) t) : expr.Expr (ident:=ident) t
-      := unfold_Rewrite (@RewriteToFancy_folded invert_low invert_high t e).
-    Definition RewriteToFancyWithCasts_folded
-               (invert_low invert_high : Z (*log2wordmax*) -> Z -> @option Z)
-               (value_range flag_range : zrange)
-      := @Make.Rewrite (fancy_with_casts_rewriter_data invert_low invert_high value_range flag_range).
-    Definition RewriteToFancyWithCasts
-               (invert_low invert_high : Z (*log2wordmax*) -> Z -> @option Z)
-               (value_range flag_range : zrange)
-               {t} (e : expr.Expr (ident:=ident) t) : expr.Expr (ident:=ident) t
-      := unfold_Rewrite (@RewriteToFancyWithCasts_folded invert_low invert_high value_range flag_range t e).
+      Tactic Notation "make_Rewriter" constr(include_interp) constr(specs) :=
+        let res := Build_RewriterT include_interp specs in refine res.
+    End Tactic.
   End RewriteRules.
-
-  Import defaults.
-
-  Definition PartialEvaluate {t} (e : Expr t) : Expr t := RewriteRules.RewriteNBE e.
 End Compilers.
